theories/zoo_persistent/parray.v
@@ -3,6 +3,8 @@ From iris.base_logic Require Import
 
 From zoo Require Import
   prelude.
+From zoo.iris.bi Require Import
+  big_op.
 From zoo.language Require Import
   notations.
 From zoo.diaframe Require Import
@@ -17,13 +19,14 @@ From zoo_persistent Require Import
 From zoo Require Import
   options.
 
-Implicit Types i : nat.
-Implicit Types l root : location.
-Implicit Types v t eq : val.
+Implicit Types b : bool.
+Implicit Types node root : location.
+Implicit Types v t equal : val.
 Implicit Types vs : list val.
+Implicit Types nodes : gmap location (list val).
 
 Class ParrayG Σ `{zoo_G : !ZooG Σ} := {
-  parray_G_map_G : ghost_mapG Σ location (list val) ;
+  parray_G_nodes_G : ghost_mapG Σ location (list val) ;
 }.
 
 Definition parray_Σ := #[
@@ -38,78 +41,90 @@ Qed.
 
 Section parray_G.
   Context `{parray_G : ParrayG Σ}.
+  Context τ `{!iType (iProp Σ) τ}.
 
   Record metadata := {
-    metadata_map : gname ;
-    metadata_array : val ;
     metadata_size : nat ;
+    metadata_data : val ;
+    metadata_nodes : gname ;
   }.
   Implicit Types γ : metadata.
 
-  #[local] Definition mapping_auth' γ_map map :=
-    @ghost_map_auth _ _ _ _ _ parray_G_map_G γ_map 1 map.
-  #[local] Definition mapping_auth γ :=
-    mapping_auth' γ.(metadata_map).
-  #[local] Definition mapping_elem' γ_map l vs :=
-    @ghost_map_elem _ _ _ _ _ parray_G_map_G γ_map l DfracDiscarded vs.
-  #[local] Definition mapping_elem γ :=
-    mapping_elem' γ.(metadata_map).
+  #[local] Definition nodes_auth' γ_nodes :=
+    @ghost_map_auth _ _ _ _ _ parray_G_nodes_G γ_nodes 1.
+  #[local] Definition nodes_auth γ :=
+    nodes_auth' γ.(metadata_nodes).
+  #[local] Definition nodes_elem' γ_nodes node :=
+    @ghost_map_elem _ _ _ _ _ parray_G_nodes_G γ_nodes node DfracDiscarded.
+  #[local] Definition nodes_elem γ :=
+    nodes_elem' γ.(metadata_nodes).
 
-  #[local] Definition inv_inner τ `{!iType _ τ} γ map root : iProp Σ :=
-    mapping_auth γ map ∗
-    [∗ map] l ↦ vs ∈ map,
-      ∃ descr,
-      ⌜length vs = γ.(metadata_size)⌝ ∗
-      l ↦ᵣ descr ∗
-      if (decide (l = root)) then (
-        ⌜descr = ‘Root( γ.(metadata_array) )%V⌝ ∗
-        array_model γ.(metadata_array) (DfracOwn 1) vs ∗
-        [∗ list] v ∈ vs, τ v
-      ) else (
-        ∃ i v l' vs',
-        ⌜i < γ.(metadata_size) ∧ vs = <[i := v]> vs'⌝ ∗
-        ⌜descr = ‘Diff( #i, v, #l' )%V⌝ ∗
-        mapping_elem γ l' vs' ∗
-        τ v
-      ).
-  Definition parray_inv τ `{!iType _ τ} γ : iProp Σ :=
-    ∃ map root,
-    inv_inner τ γ map root.
+  #[local] Definition node_model γ node vs : iProp Σ :=
+    ∃ (i : nat) v node' vs',
+    node ↦ᵣ ‘Diff( #i, v, #node' ) ∗
+    τ v ∗
+    nodes_elem γ node' vs' ∗
+    ⌜length vs = γ.(metadata_size)⌝ ∗
+    ⌜i < γ.(metadata_size)⌝ ∗
+    ⌜vs = <[i := v]> vs'⌝.
+  #[local] Instance : CustomIpatFormat "node_model" :=
+    "(
+      %i_{node} &
+      %v_{node} &
+      %node{='} &
+      %vs_node{='} &
+      H{node}{_{suff}} &
+      #Hv_{node} &
+      #Hnodes_elem_node{='} &
+      % &
+      % &
+      %Hvs_{node}
+    )".
+  #[local] Definition inv' γ nodes root : iProp Σ :=
+    ∃ vs_root,
+    nodes_auth γ nodes ∗
+    root ↦ᵣ ‘Root( γ.(metadata_data) ) ∗
+    array_model γ.(metadata_data) (DfracOwn 1) vs_root ∗
+    ⌜nodes !! root = Some vs_root⌝ ∗
+    ⌜length vs_root = γ.(metadata_size)⌝ ∗
+    ([∗ list] v ∈ vs_root, τ v) ∗
+    [∗ map] node ↦ vs ∈ delete root nodes,
+      node_model γ node vs.
+  #[local] Instance : CustomIpatFormat "inv'" :=
+    "(
+      %vs_{root} &
+      Hnodes_auth &
+      H{root} &
+      Hdata &
+      %Hnodes_lookup_{root} &
+      % &
+      #Hvs_{root} &
+      Hnodes
+    )".
+  Definition parray_inv γ : iProp Σ :=
+    ∃ nodes root,
+    inv' γ nodes root.
+  #[local] Instance : CustomIpatFormat "inv" :=
+    "(
+      %nodes &
+      %{root} &
+      (:inv')
+    )".
 
   Definition parray_model t γ vs : iProp Σ :=
-    ∃ l,
-    ⌜t = #l⌝ ∗
-    mapping_elem γ l vs.
+    ∃ node,
+    ⌜t = #node⌝ ∗
+    nodes_elem γ node vs.
+  #[local] Instance : CustomIpatFormat "model" :=
+    "(
+      %node &
+      -> &
+      #Hnodes_elem_node
+    )".
 
-  #[local] Instance inv_inner_timeless τ `{!iType _ τ} γ map root :
+  #[global] Instance parray_inv_timeless γ :
     (∀ v, Timeless (τ v)) →
-    Timeless (inv_inner τ γ map root).
-  Proof.
-    rewrite /Timeless. iIntros "%Hτ (Hmap_auth & Hmap)".
-    iSplitL "Hmap_auth".
-    - iApply (timeless with "Hmap_auth").
-    - unshelve iApply (timeless _ (Timeless := big_sepM_timeless _ _ _) with "Hmap").
-      rewrite /Timeless. iIntros "%l %vs _ (%descr & >%Hvs_len & Hl & Hdescr)".
-      iExists descr.
-      iSplit; first iSteps.
-      iSplitL "Hl"; first iApply (timeless with "Hl").
-      case_decide as Hcase.
-      + iDestruct "Hdescr" as "(>-> & Harr & Hvs)".
-        iSplit; first iSteps.
-        iSplitL "Harr"; first iApply (timeless with "Harr").
-        unshelve iApply (timeless _ (Timeless := big_sepL_timeless _ _ _) with "Hvs").
-        rewrite /Timeless. iIntros "%i %v _ Hv".
-        iApply (Hτ with "Hv").
-      + iDestruct "Hdescr" as "(%i & %v & %l' & %vs' & >(%Hi & %Hvs) & >-> & Hmap_elem' & Hv)".
-        iExists i, v, l', vs'.
-        iSplit; first iSteps.
-        iSplit; first iSteps.
-        iSplit; first iApply (timeless with "Hmap_elem'").
-        iApply (Hτ with "Hv").
-  Qed.
-  #[global] Instance parray_inv_timeless τ `{!iType _ τ} γ :
-    (∀ v, Timeless (τ v)) →
-    Timeless (parray_inv τ γ).
+    Timeless (parray_inv γ).
   Proof.
     apply _.
   Qed.
@@ -124,37 +139,37 @@ Section parray_G.
     apply _.
   Qed.
 
-  #[local] Lemma mapping_alloc root vs :
+  #[local] Lemma nodes_alloc root vs :
     ⊢ |==>
-      ∃ γ_map,
-      mapping_auth' γ_map {[root := vs]} ∗
-      mapping_elem' γ_map root vs.
+      ∃ γ_nodes,
+      nodes_auth' γ_nodes {[root := vs]} ∗
+      nodes_elem' γ_nodes root vs.
   Proof.
-    iMod (@ghost_map_alloc _ _ _ _ _ parray_G_map_G {[root := vs]}) as "(%γ_map & Hmap_auth & Hmap_elem)".
-    setoid_rewrite big_sepM_singleton.
-    iMod (ghost_map_elem_persist with "Hmap_elem") as "Hmap_elem".
+    iMod (@ghost_map_alloc _ _ _ _ _ parray_G_nodes_G {[root := vs]}) as "(%γ_nodes & Hnodes_auth & Hnodes_elem)".
+    rewrite big_sepM_singleton.
+    iMod (ghost_map_elem_persist with "Hnodes_elem") as "Hnodes_elem".
     iSteps.
   Qed.
-  #[local] Lemma mapping_lookup γ map l vs :
-    mapping_auth γ map -∗
-    mapping_elem γ l vs -∗
-    ⌜map !! l = Some vs⌝.
+  #[local] Lemma nodes_lookup γ nodes node vs :
+    nodes_auth γ nodes -∗
+    nodes_elem γ node vs -∗
+    ⌜nodes !! node = Some vs⌝.
   Proof.
     apply ghost_map_lookup.
   Qed.
-  #[local] Lemma mapping_insert {γ map} l vs :
-    map !! l = None →
-    mapping_auth γ map ⊢ |==>
-      mapping_auth γ (<[l := vs]> map) ∗
-      mapping_elem γ l vs.
+  #[local] Lemma nodes_insert {γ nodes} node vs :
+    nodes !! node = None →
+    nodes_auth γ nodes ⊢ |==>
+      nodes_auth γ (<[node := vs]> nodes) ∗
+      nodes_elem γ node vs.
   Proof.
-    iIntros "%Hlookup Hmap_auth".
-    iMod (ghost_map_insert with "Hmap_auth") as "(Hmap_auth & Hmap_elem)"; first done.
-    iMod (ghost_map_elem_persist with "Hmap_elem") as "Hmap_elem".
+    iIntros "%Hlookup Hnodes_auth".
+    iMod (ghost_map_insert with "Hnodes_auth") as "(Hnodes_auth & Hnodes_elem)"; first done.
+    iMod (ghost_map_elem_persist with "Hnodes_elem") as "Hnodes_elem".
     iSteps.
   Qed.
 
-  Lemma parray_make_spec τ `{!iType _ τ} (sz : Z) v :
+  Lemma parray_make_spec (sz : Z) v :
     (0 ≤ sz)%Z →
     {{{
       τ v
@@ -162,163 +177,213 @@ Section parray_G.
       parray_make #sz v
     {{{ t γ,
       RET t;
-      parray_inv τ γ ∗
+      parray_inv γ ∗
       parray_model t γ (replicate ₊sz v)
     }}}.
   Proof.
     iIntros "%Hsz %Φ #Hv HΦ".
+
     wp_rec.
-    wp_smart_apply (array_unsafe_make_spec with "[//]") as "%arr Harr"; first done.
+    wp_smart_apply (array_unsafe_make_spec with "[//]") as "%data Hdata"; first done.
     wp_ref root as "Hroot".
-    pose vs := replicate ₊sz v.
-    iMod (mapping_alloc root vs) as "(%γ_map & Hmap_auth & Hmap_elem)".
+
+    iMod (nodes_alloc root (replicate ₊sz v)) as "(%γ_nodes & Hnodes_auth & Hnodes_elem)".
+
     pose γ := {|
-      metadata_map := γ_map ;
-      metadata_array := arr ;
       metadata_size := ₊sz ;
+      metadata_data := data ;
+      metadata_nodes := γ_nodes ;
     |}.
-    iApply ("HΦ" $! _ γ). iSplitR "Hmap_elem"; last iSteps. iExists {[root := vs]}, root. iFrame.
-    iApply big_sepM_singleton.
-    iExists _. rewrite length_replicate decide_True //. iSteps.
-    iApply big_sepL_intro. iIntros "!> !>" (i ? (-> & Hi)%lookup_replicate) "//".
+
+    iApply ("HΦ" $! _ γ).
+    iModIntro. iFrame.
+    rewrite lookup_insert length_replicate delete_singleton big_sepM_empty.
+    rewrite big_op.big_sepL_replicate -big_sepL_intro.
+    auto 10.
   Qed.
 
-  #[local] Lemma parray_reroot_spec τ `{!iType _ τ} γ map root l vs :
+  #[local] Definition reroot_inv γ nodes root vs_root : iProp Σ :=
+    ∃ descr_root,
+    nodes_auth γ nodes ∗
+    root ↦ᵣ descr_root ∗
+    array_model γ.(metadata_data) (DfracOwn 1) vs_root ∗
+    ⌜length vs_root = γ.(metadata_size)⌝ ∗
+    ([∗ list] v ∈ vs_root, τ v) ∗
+    [∗ map] node ↦ vs ∈ delete root nodes,
+      node_model γ node vs.
+  #[local] Instance : CustomIpatFormat "reroot_inv" :=
+    "(
+      %descr_{root} &
+      Hnodes_auth &
+      H{root} &
+      Hdata &
+      % &
+      #Hvs_{root} &
+      Hnodes
+    )".
+  #[local] Lemma parray_reroot_0_spec {γ nodes root node} vs :
     {{{
-      inv_inner τ γ map root ∗
-      mapping_elem γ l vs
+      inv' γ nodes root ∗
+      nodes_elem γ node vs
     }}}
-      parray_reroot #l
+      parray_reroot_0 #node
     {{{
-      RET γ.(metadata_array);
-      inv_inner τ γ map l
+      RET γ.(metadata_data);
+      reroot_inv γ nodes node vs
     }}}.
   Proof.
-    iLöb as "HLöb" forall (l vs).
-    iIntros "%Φ ((Hmap_auth & Hmap) & #Hmap_elem) HΦ".
+    iLöb as "HLöb" forall (node vs).
+
+    iIntros "%Φ ((:inv') & #Hnodes_elem_node) HΦ".
+
     wp_rec.
-    iDestruct (mapping_lookup with "Hmap_auth Hmap_elem") as %Hmap_lookup.
-    iDestruct (big_sepM_lookup_acc with "Hmap") as "((%descr & %Hvs_len & Hl & Hdescr) & Hmap)"; first done.
-    destruct (decide (l = root)) as [-> | Hcase1].
-    { iDestruct "Hdescr" as "(-> & Harr & Hvs)". iSteps. }
-    iDestruct "Hdescr" as "(%i & %v & %l' & %vs' & (%Hi & %Hvs) & -> & #Hmap_elem' & #Hv)".
-    wp_load.
-    iDestruct ("Hmap" with "[Hl Hv]") as "Hmap"; first iSteps.
-    wp_smart_apply ("HLöb" with "[Hmap_auth Hmap]") as "(Hmap_auth & Hmap)"; first iSteps.
-    wp_pures.
-    iDestruct (mapping_lookup with "Hmap_auth Hmap_elem'") as %Hmap_lookup'.
-    iDestruct (big_sepM_delete with "Hmap") as "((%descr' & %Hvs'_len & Hl' & Hdescr') & Hmap)"; first done.
-    rewrite decide_True //. iDestruct "Hdescr'" as "(-> & Harr & Hvs')".
-    opose proof* (list_lookup_lookup_total_lt vs' i) as Hvs'_lookup; first lia.
-    wp_apply (array_unsafe_get_spec i with "Harr") as "Harr"; [lia | | lia |]; first done.
-    wp_store.
-    wp_smart_apply (array_unsafe_set_spec with "Harr") as "Harr"; first lia.
-    rewrite Nat2Z.id -Hvs.
-    destruct (decide (l = l')) as [<- | Hcase2].
-    - wp_store.
-      iDestruct (big_sepM_delete with "[$Hmap Hl' Harr Hvs']") as "Hmap"; first done.
-      { iExists _. rewrite decide_True //. clear Hvs. simplify. iSteps. }
+    destruct (decide (node = root)) as [-> | Hnode].
+
+    - iDestruct (nodes_lookup with "Hnodes_auth Hnodes_elem_node") as %Hnodes_lookup_root_. simplify.
       iSteps.
-    - iDestruct (big_sepM_delete _ _ l with "Hmap") as "((%descr & _ & Hl & Hdescr) & Hmap)"; first rewrite lookup_delete_ne //.
-      rewrite decide_False //. iDestruct "Hdescr" as "(%i'' & %w & %l'' & %vs'' & _ & -> & _ & _)".
-      wp_store. wp_pures.
-      iApply "HΦ". iFrame.
-      iDestruct (big_sepL_insert_acc with "Hvs'") as "(Hvs'!!!i & Hvs')"; first done.
-      iApply (big_sepM_delete _ _ l'); first done. iSplitL "Hl' Hvs'!!!i".
-      { iExists _. rewrite decide_False //. iFrame. iSplitR; first iSteps. iExists i, l, vs. iSteps.
-        iPureIntro. rewrite Hvs list_insert_insert list_insert_id //.
+
+    - iDestruct (nodes_lookup with "Hnodes_auth Hnodes_elem_node") as %Hnodes_lookup_node.
+      iDestruct (big_sepM_lookup_acc with "Hnodes") as "((:node_model =1) & Hnodes)".
+      { rewrite lookup_delete_ne //. }
+      wp_load.
+
+      wp_smart_apply ("HLöb" $! node1 vs_node1 with "[- HΦ]") as "(:reroot_inv root=node1)"; first iFrameSteps.
+
+      destruct (lookup_lt_is_Some_2 vs_node1 i_node) as (v & Hvs_node1_lookup); first lia.
+      wp_smart_apply (array_unsafe_get_spec with "Hdata") as "Hdata"; [lia | done | lia |].
+      wp_store.
+      wp_smart_apply (array_unsafe_set_spec with "Hdata") as "Hdata"; first lia.
+      rewrite Nat2Z.id -Hvs_node.
+      wp_pures.
+
+      iDestruct (big_sepL_insert i_node with "Hvs_node1 Hv_node") as "Hvs"; first lia.
+      rewrite -Hvs_node.
+
+      iDestruct (nodes_lookup with "Hnodes_auth Hnodes_elem_node1") as %Hnodes_lookup_node1.
+      iDestruct (big_sepM_delete_2 with "Hnodes [$Hnode1]") as "Hnodes"; first done.
+      { iDestruct (big_sepL_lookup with "Hvs_node1") as "$"; first done.
+        iSteps. iPureIntro.
+        rewrite Hvs_node list_insert_insert list_insert_id //.
       }
-      iApply (big_sepM_delete _ _ l); first rewrite lookup_delete_ne //. iSplitL "Hl Harr Hvs'".
-      { iExists _. rewrite decide_True //.
-        iSpecialize ("Hvs'" $! v). rewrite -Hvs.
-        iSteps.
-      }
-      iApply (big_sepM_impl with "Hmap"). clear. iIntros "!> !>" (l'' vs'' (Hl''1 & (Hl''2 & Hmap_lookup'')%lookup_delete_Some)%lookup_delete_Some) "(%descr'' & %Hvs''_len & Hl'' & Hdescr'')".
-      iExists _. rewrite decide_False // decide_False //. iFrameSteps.
+      iClear "Hv_node". clear dependent i_node v_node.
+      iDestruct (big_sepM_delete_1 node with "Hnodes") as "((:node_model =2) & Hnodes)"; first done.
+
+      iSteps.
+  Qed.
+  #[local] Lemma parray_reroot_spec γ node vs :
+    {{{
+      parray_inv γ ∗
+      nodes_elem γ node vs
+    }}}
+      parray_reroot #node
+    {{{ nodes,
+      RET γ.(metadata_data);
+      inv' γ nodes node
+    }}}.
+  Proof.
+    iIntros "%Φ ((:inv) & #Hnodes_elem_node) HΦ".
+
+    wp_rec.
+    destruct (decide (node = root)) as [-> | Hnode]; first iSteps.
+
+    iDestruct (nodes_lookup with "Hnodes_auth Hnodes_elem_node") as %Hnodes_lookup_node.
+    iDestruct (big_sepM_lookup_acc with "Hnodes") as "((:node_model) & Hnodes)".
+    { rewrite lookup_delete_ne //. }
+    wp_load.
+
+    wp_smart_apply (parray_reroot_0_spec vs with "[- HΦ]") as "(:reroot_inv root=node)"; first iFrameSteps.
+    iSteps.
   Qed.
 
-  Lemma parray_get_spec τ `{!iType _ τ} {t γ vs} {i : Z} v :
+  Lemma parray_get_spec {t γ vs} i v :
     (0 ≤ i)%Z →
     vs !! ₊i = Some v →
     {{{
-      parray_inv τ γ ∗
+      parray_inv γ ∗
       parray_model t γ vs
     }}}
       parray_get t #i
     {{{
       RET v;
-      parray_inv τ γ
+      parray_inv γ
     }}}.
   Proof.
-    iIntros "%Hi %Hvs_lookup %Φ ((%map & %root & Hinv) & (%l & -> & #Hmap_elem)) HΦ".
+    iIntros "% %Hvs_lookup %Φ (Hinv & (:model)) HΦ".
+
     wp_rec.
-    wp_smart_apply (parray_reroot_spec τ with "[$Hinv $Hmap_elem]") as "(Hmap_auth & Hmap)".
-    iDestruct (mapping_lookup with "Hmap_auth Hmap_elem") as %Hmap_lookup.
-    iDestruct (big_sepM_lookup_acc with "Hmap") as "((%descr & %Hvs_len & Hl & Hdescr) & Hmap)"; first done.
-    rewrite decide_True //. iDestruct "Hdescr" as "(-> & Harr & Hvs)".
-    wp_apply (array_unsafe_get_spec with "Harr"); [done.. |].
-    setoid_rewrite decide_True at 1; last done. iSteps.
+    wp_smart_apply (parray_reroot_spec with "[$Hinv $Hnodes_elem_node]") as (nodes) "(:inv' root=node)".
+
+    iDestruct (nodes_lookup with "Hnodes_auth Hnodes_elem_node") as %Hnodes_lookup_node_. simplify.
+    wp_smart_apply (array_unsafe_get_spec with "Hdata") as "Hdata"; [done.. |].
+
+    iStepFrameSteps.
   Qed.
 
-  Lemma parray_set_spec τ `{!iType _ τ} t γ vs eq (i : Z) v :
+  Lemma parray_set_spec t γ vs equal i v :
     (0 ≤ i < length vs)%Z →
     {{{
-      parray_inv τ γ ∗
+      parray_inv γ ∗
       parray_model t γ vs ∗
       ( ∀ v1 v2,
         τ v1 -∗
         τ v2 -∗
-        WP eq v1 v2 {{ res,
-          ⌜res = #(bool_decide (v1 = v2))⌝
+        WP equal v1 v2 {{ res,
+          ∃ b,
+          ⌜res = #b⌝ ∗
+          ⌜if b then v1 = v2 else True⌝
         }}
       ) ∗
       τ v
     }}}
-      parray_set t eq #i v
+      parray_set t equal #i v
     {{{ t',
       RET t';
-      parray_inv τ γ ∗
+      parray_inv γ ∗
       parray_model t' γ (<[₊i := v]> vs)
     }}}.
   Proof.
-    iIntros "%Hi %Φ ((%map & %root & Hinv) & (%l & -> & #Hmap_elem) & Heq & #Hv) HΦ".
-    Z_to_nat i. rewrite Nat2Z.id.
+    iIntros "% %Φ (Hinv & (:model) & Hequal & #Hv) HΦ".
+
     wp_rec.
-    wp_smart_apply (parray_reroot_spec with "[$Hinv //]") as "(Hmap_auth & Hmap)".
-    iDestruct (mapping_lookup with "Hmap_auth Hmap_elem") as %Hmap_lookup.
-    iDestruct (big_sepM_delete _ _ l with "Hmap") as "((%descr & %Hvs_len & Hl & Hdescr) & Hmap)"; first done.
-    rewrite decide_True //. iDestruct "Hdescr" as "(-> & Harr & Hvs)".
-    opose proof* (list_lookup_lookup_total_lt vs i); first lia.
-    wp_smart_apply (array_unsafe_get_spec i with "Harr") as "Harr"; [lia | done | lia |].
-    iDestruct (big_sepL_insert_acc with "Hvs") as "(#Hvs!!!i & Hvs)"; first done.
-    wp_smart_apply (wp_wand with "(Heq Hv Hvs!!!i)") as "% ->".
-    wp_pures. case_bool_decide as Hcase; wp_pures.
-    - iDestruct ("Hvs" with "Hv") as "Hvs".
-      rewrite list_insert_id; first congruence.
-      iDestruct (big_sepM_delete with "[Hl Harr Hvs $Hmap]") as "Hmap"; first done.
-      { iExists _. rewrite decide_True //. iSteps. }
-      iSteps.
-    - wp_apply (array_unsafe_set_spec with "Harr") as "Harr"; first done. rewrite Nat2Z.id.
-      wp_load. clear root. wp_ref root as "Hroot". wp_store. wp_pures.
-      iApply "HΦ".
-      iAssert ⌜map !! root = None⌝%I as %Hmap_lookup_root.
-      { rewrite -eq_None_ne_Some. iIntros "%vs_root %Hmap_lookup_root".
-        iDestruct (pointsto_ne with "Hroot Hl") as %Hne.
-        iDestruct (big_sepM_lookup _ _ root with "Hmap") as "(%descr & _ & Hroot_ & _)".
+    wp_smart_apply (parray_reroot_spec with "[$Hinv $Hnodes_elem_node]") as (nodes) "(:inv' root=node)".
+
+    iDestruct (nodes_lookup with "Hnodes_auth Hnodes_elem_node") as %Hnodes_lookup_node_. simplify.
+    destruct (lookup_lt_is_Some_2 vs_node ₊i) as (w & Hvs_node_lookup); first lia.
+    wp_smart_apply (array_unsafe_get_spec with "Hdata") as "Hdata"; [done.. |].
+
+    iDestruct (big_sepL_lookup with "Hvs_node") as "#Hw"; first done.
+    wp_smart_apply (wp_wand with "(Hequal Hv Hw)") as (res) "(%b & -> & %Hb)".
+    destruct b; first subst w; wp_pures.
+
+    - rewrite list_insert_id //.
+      iStepFrameSteps.
+
+    - wp_apply (array_unsafe_set_spec with "Hdata") as "Hdata"; first done.
+      wp_load.
+      wp_ref root as "Hroot".
+      wp_store. wp_pures.
+
+      iAssert ⌜nodes !! root = None⌝%I as %Hnodes_lookup_root.
+      { rewrite -eq_None_ne_Some. iIntros "%vs_root %Hnodes_lookup_root".
+        iDestruct (pointsto_ne with "Hroot Hnode") as %?.
+        iDestruct (big_sepM_lookup _ _ root with "Hnodes") as "(:node_model node=root suff=)".
         { rewrite lookup_delete_ne //. congruence. }
         iApply (pointsto_exclusive with "Hroot Hroot_").
       }
-      set vs_root := <[i := v]> vs.
-      iMod (mapping_insert with "Hmap_auth") as "(Hmap_auth & #Hmap_elem_root)"; first done.
-      iSplitR "Hmap_elem_root"; last iSteps. iExists (<[root := vs_root]> map), root. iFrame.
-      iApply big_sepM_insert; first done. iSplitL "Hroot Harr Hvs".
-      { iExists _. rewrite decide_True //. iSteps. rewrite length_insert //. }
-      iApply (big_sepM_delete _ _ l); first done. iSplitL "Hl".
-      { iExists _. rewrite decide_False; first congruence. iStep 2. iExists i, (vs !!! i), root, vs_root. iSteps.
-        iPureIntro. rewrite /vs_root list_insert_insert list_insert_id //.
+
+      set vs_root := <[₊i := v]> vs_node.
+      iDestruct (big_sepL_insert ₊i with "Hvs_node Hv") as "Hvs_root"; first lia.
+      iMod (nodes_insert root vs_root with "Hnodes_auth") as "(Hnodes_auth & #Hnodes_elem_root)"; first done.
+      iDestruct (big_sepM_insert_delete_2 with "Hnodes [Hnode]") as "Hnodes".
+      { iExists ₊i, w, root, vs_root. iSteps; iPureIntro.
+        - rewrite Z2Nat.id //.
+        - rewrite list_insert_insert list_insert_id //.
       }
-      iApply (big_sepM_impl with "Hmap"). iIntros "!> !>" (l' vs'' (Hne & Hmap_lookup')%lookup_delete_Some) "(%descr' & %Hvs'_len & Hl' & Hdescr')".
-      iExists _. rewrite decide_False // decide_False; first congruence. iFrameSteps.
+      iEval (rewrite insert_id //) in "Hnodes".
+      rewrite -{2}(delete_insert nodes root vs_root) //.
+      iStepFrameSteps; iPureIntro.
+      { rewrite lookup_insert //. }
+      { rewrite /vs_root. simpl_length. }
   Qed.
 End parray_G.
 
